Switch the top-level MLS API to the target simplfied API

fstar/new/MLS.fsti
@@ -1,102 +1,44 @@
+/// A revised version of the top-level MLS API exposed to clients.
+///
+/// This is a simplified version that does not expose a notion of commit.
+/// Furthermore, we assume that the user is online for all of the group
+/// modifications.
 module MLS
 
-// The user-friendy API for MLS. This is the set of functions we expose outside
-// of the library.
+val group_id: Type0
+val participant_id: Type0
+val state: group_id -> Type0
 
-// JP: What does the credential represent? How does one obtain a credential? Right
-// now there is now way to obtain a credential, and thus no way to call `create`.
-val credential: Type0
-// JP: Same remark.
-val enc_key: Type0
+let bytes = MLS.Lib.Array.array Lib.IntTypes.uint8
+let group_message = group_id & bytes
+let welcome_message = participant_id & bytes
 
-// JP: Why not Array.length? Why does this need to be in the API?
-val length: array 'a -> nat
+// JP: any further changes?
+let entropy = bytes
 
-// JP: Why hide this? Is this an array of u8, a sequence, or FStar.Bytes.bytes?
-val bytes: Type0
-
-(* Public Information about a Group Member *)
-noeq type member_info = {
-  cred: credential;
-  version: nat;
-  current_enc_key: enc_key
+noeq
+type public_info = {
+  public_key: bytes;
+  user_id: participant_id;
 }
 
-(* Secrets belonging to a Group Member. *)
-// JP: No way to create a `member_secrets`, meaning no way to call
-// `generate_commit_and_welcome`
-val member_secrets: Type0
-
-(* Group State Data Structure *)
-val group_state: Type0
-
-val group_id: group_state → nat
-val group_size: group_state → nat
-val epoch: group_state → nat
-type index (g:group_state) = i:nat{i < group_size g}
-
-type member_array (sz:nat) = a:array (option member_info){length a = sz}
-
-// JP: Is this going to generate un-necessary copies? Can we do something smarter,
-// e.g. request a member at index i? (Maybe doesn't matter, not sure.)
-val membership: g:group_state → member_array (group_size g)
-
-(* Create a new Group State *)
-// JP: need to document why the option might be empty.
-// JP: what is a `gid`? how is it chosen?
-// JP: why does the creator have a distinguished status? can't we offer a "fresh
-// group" operation that returns a new empty group (with a suitably-chosen id),
-// then apply an `add` operation to add the initiator to the group?
-val create: gid:nat → creator_mi:member_info → entropy:bytes → option group_state
-
-(* Group Operation Data Structure *)
-// JP: missing API to create an update_path, so can't create a commit, so can't call apply.
-val update_path: Type0
-
-noeq type operation =
-  | Add: member_info -> operation
-  // JP: should all of these `nat`s be `uint32` rather? having Zarith sent
-  // across language boundaries is going to be a nightmare
-  | Update: nat -> member_info -> operation
-  | Remove: nat -> operation
-
-noeq type commit = {
-  operations: list operation;
-  update_path: option update_path;
+noeq
+type private_info = {
+  private_key: bytes;
+  user_id: participant_id;
 }
 
-// JP: why separate encryption state and group state? does the user need to
-// distinguish between the two?
-val encryption_state: Type0
+// TODO: expose a way to inject e.g. a uint32 into a group_id
+val create: entropy → private_info → g:group_id -> state g
 
-(* Apply an Operation to a Group *)
-val apply: (group_state & encryption_state) → commit → option (group_state & encryption_state)
+val add: #g:group_id -> state g → public_info → group_message & welcome_message
 
-(* Protocol Messages *)
-noeq type msg =
-| AppMsg: ctr:nat → m:bytes → msg
-| Commit: commit → msg
-| Goodbye: msg
+val remove: #g:group_id -> state g → public_info → group_message
 
-type welcome_message
+val update: #g:group_id -> state g → entropy → group_message
 
-// JP: Can the welcome be generated independently of the commit, and at any
-// time? This API feels a bit bizarre. I'm also confused by what the index
-// stands for, and why the *user* needs to maintain member_secrets
-val generate_commit_and_welcome: g:group_state -> encryption_state -> list operation -> entropy:bytes -> index g -> member_secrets -> (commit & option welcome_message)
+// To send application data
+val send: #g:group_id -> state g → entropy → bytes → state g & group_message
 
-// JP: why does the user need to know about this?
-val get_ratchet_tree: group_state -> bytes
-
-// JP: Why this two-step API? Why not generate_welcome: state -> bytes and process_welcome: bytes -> state?
-val serialize_welcome_message: welcome_message -> bytes
-
-val deserialize_welcome_message: bytes -> welcome_message
-
-val unpack_welcome: welcome_message -> (group_state & encryption_state)
-
-(* Encrypt Protocol Message *)
-val encrypt_msg: g:group_state → es:encryption_state → sender:index g → m:msg → entropy:bytes → (bytes * encryption_state)
-(* Decrypt Protocol Message *)
-val decrypt_msg: g:group_state → es:encryption_state → receiver:index g → c:bytes → option (msg * sender:index g * encryption_state)
-
+val process_welcome_message: welcome_message → (g:group_id & state g)
+val process_group_message: #g:group_id -> state g → group_message → (state g & option bytes)
